cleaned up some definitions and proofs for simulation

LTS.thy
@@ -12,7 +12,7 @@ text {* The semantics of a B component is a discrete, eventful, state-transition
 first define what is meant exactly by such systems. Any system is, at a given time in a state. 
 Conversely, a system has a set of possible states. A system evolves from state to state,
 and such changes called transitions. The following record definition of 
-@{text "('st, 'ev) Transition}"} models transitions, where the parametric sorts @{text "'st"} 
+@{text "('st, 'ev) Tr}"} models transitions, where the parametric sorts @{text "'st"} 
 and @{text "'ev"} represent states and events, respectively. *}
 
 record ('st, 'ev) Tr =
@@ -45,7 +45,7 @@ We first define a function @{text "successors"} that returns the set of successo
 given set @{text "S"} of states in a given LTS @{text "L"}: *}
 
 definition successors :: "('st, 'ev) LTS \<Rightarrow> 'st set \<Rightarrow> 'st set" where
-"successors L S \<equiv> { s | s . \<exists> t \<in> trans L. src t \<in> S \<and> dst t = s}"
+  "successors m S \<equiv> { dst t | t . t \<in> trans m \<and> src t \<in> S }"
 
 text {* Next, we show that the successors of the reachable states are also reachable. *}
 
@@ -58,50 +58,41 @@ states are in $S$, and if the successors of $S$ are in $S$ then all the reachabl
 $S$. *}
 
 lemma reachable_induct_set:
-  assumes base: "init m \<subseteq> S" and step: "successors m S \<subseteq> S"
-  shows "(states m) \<subseteq> S"
-proof
-  fix x
-  assume "x \<in> states m"
-  thus "x \<in> S"
-  proof (induct x)
-    fix i
-    assume "i \<in> init m"
-    with base show "i \<in> S" ..
-  next
-    fix t
-    assume "t \<in> trans m" "src t \<in> states m" "src t \<in> S"
-    with step show "dst t \<in> S" unfolding successors_def by auto
-  qed
+  assumes s: "s \<in> states m" and base: "init m \<subseteq> S" and step: "successors m S \<subseteq> S"
+  shows "s \<in> S"
+using s proof (induct s)
+  fix i
+  assume "i \<in> init m"
+  with base show "i \<in> S" ..
+next
+  fix t
+  assume "t \<in> trans m" and "src t \<in> S"
+  with step show "dst t \<in> S" unfolding successors_def by auto
 qed
 
-text {* Next we enunciate and prove a similar lemma for predicates. In a LTS @{text "L"}, 
+text {* Next we enunciate and prove a similar lemma for predicates. In a LTS @{text "m"}, 
 if every initial state
 statisfies some predicate @{text "P"} and, for each transition, whenever the source state
 satisfies @{text "P"}, the destination state also satisfies @{text "P"}, then all the
 reachable states satisfy @{text "P"} (and this is an invariant of the LTS). *}
 lemma reachable_induct_predicate:
-  assumes base: "\<forall> s \<in> init L . P s" and 
-          step: "\<forall> t \<in> trans L . P (src t) \<longrightarrow> P (dst t)"
-  shows "\<forall> s \<in> (states L) . P s"
-proof
-  fix x
-  assume "x \<in> states L" 
-  thus "P x"
-  proof (induct x)
-    fix i
-    assume "i \<in> init L"
-    with base show "P i" ..
+  assumes s: "s \<in> states m"
+      and base: "\<forall>s \<in> init m. P s"
+      and step: "\<forall>t \<in> trans m. P (src t) \<longrightarrow> P (dst t)"
+  shows "P s"
+proof -
+  from s have "s \<in> { s . P s}" (is "s \<in> ?S")
+  proof (rule reachable_induct_set)
+    from base show "init m \<subseteq> ?S" by auto
   next
-    fix t
-    assume "t \<in> trans L" "src t \<in> states L" "P (src t)"
-    with step show "P (dst t)" unfolding successors_def by auto
+    from step show "successors m ?S \<subseteq> ?S" by (auto simp: successors_def)
   qed
+  thus ?thesis ..
 qed
 
 subsection {* Behavior *}
 
-subsubsection {* Internal behaviour *}
+subsubsection {* Internal behavior *}
 
 text {* Two views of behavior are formalized. The first view is the internal behavior, and
 corresponds to the set of possible executions. An execution is a sequence of transitions, such
@@ -115,28 +106,22 @@ denotes all possible executions of a given LTS @{text "L"}. There are two base c
 corresponding to the empty execution and to executions with a single transition: *}
 
 inductive_set runs :: "('st, 'ev) LTS \<Rightarrow> ('st, 'ev) Run set"  
-          for L :: "('st, 'ev) LTS" where
-  base: "[] \<in> runs L"
-| start: "\<lbrakk> t \<in> trans L; src t \<in> init L \<rbrakk> \<Longrightarrow> [t] \<in> runs L"
-| step: "\<lbrakk> t \<in> trans L; r \<noteq> []; r \<in> runs L; src t = dst (last r) \<rbrakk> \<Longrightarrow> r @ [t] \<in> runs L"
+          for m :: "('st, 'ev) LTS" where
+  base: "[] \<in> runs m"
+| start: "\<lbrakk> t \<in> trans m; src t \<in> init m \<rbrakk> \<Longrightarrow> [t] \<in> runs m"
+| step: "\<lbrakk> t \<in> trans m; ts \<in> runs m; ts \<noteq> []; src t = dst (last ts) \<rbrakk> \<Longrightarrow> ts @ [t] \<in> runs m"
 
 inductive_cases empty_run : "[] \<in> runs m"
 inductive_cases one_step_run : "[t] \<in> runs m"
-inductive_cases multi_step_run : "r @ [t] \<in> runs m"
+inductive_cases multi_step_run : "ts @ [t] \<in> runs m"
 
-lemma 
-assumes "t \<in> trans L \<and> src t \<in> init L"
-shows "[t] \<in> runs L"
-by (metis assms runs.start)
-
-text {* The following lemma states that for any run $r$ of a LTS $m$, such that $r$ is not the 
+text {* The following lemma states that for any run $ts$ of a LTS $m$, such that $ts$ is not the 
 empty run, then the source state of the first transition is an initial state of $m$. *}
 
-lemma "r \<in> runs m \<Longrightarrow> r \<noteq> [] \<Longrightarrow> src(hd r) \<in> init m"
-proof(induct rule: runs.induct, auto)
-qed
+lemma "ts \<in> runs m \<Longrightarrow> ts \<noteq> [] \<Longrightarrow> src (hd ts) \<in> init m"
+by (induct rule: runs.induct) auto
 
-subsubsection {* External behavior. *}
+subsubsection {* External behavior *}
 
 text {* The external, or observable, behavior of a LTS is restricted to the events labeling its 
 transitions. We give the name @{text "Trace"} to the type of event lists: *}
@@ -145,15 +130,13 @@ type_synonym 'ev Trace = "'ev list"
 
 text {* We define the \emph{trace} of a run to be the sequence of events along that run: *}
 
-fun "trace_of_run" :: "('st, 'ev) Run \<Rightarrow> 'ev Trace" 
-where
-"trace_of_run [] = []" |
-"trace_of_run (t # ts) = (lbl t) # (trace_of_run ts)"
+definition trace_of_run :: "('st, 'ev) Run \<Rightarrow> 'ev Trace" where
+  "trace_of_run ts = map lbl ts"
 
 text {* We then define the \emph{traces} of an LTS from the corresponding runs: *}
 
 definition traces :: "('st, 'ev) LTS \<Rightarrow> 'ev Trace set" where
-  "traces m \<equiv> { trace_of_run r | r . r \<in> runs m }"
+  "traces m \<equiv> trace_of_run ` (runs m)"
 
 end
 
