ROOT
@@ -1,7 +1,12 @@
+(***********************************************************
+   Use a command such as 
+      isabelle build -D .
+   to produce the pdf document for these theories.
+***********************************************************)
+
 session "b-means" = "HOL" +
-  options [ quick_and_dirty = true, document = pdf, document_output = "output", document_variants="document:outline=/proof,/theory" ]
-  theories [document = false]
-    (* Foo Bar *)
+  options [ (*quick_and_dirty = true,*) document = pdf, document_output = "output", document_variants="document:outline=/proof,/theory" ]
+(*  theories [document = false] *)
   theories
     LTS Simulation TraceRefinement
   files "document/root.tex"
